F_mu_ref_par/examples/counter.v
@@ -1,0 +1,402 @@
+From iris.proofmode Require Import invariants ghost_ownership tactics.
+From F_mu_ref_par Require Import lang examples.lock typing
+     logrel_binary fundamental_binary rules_binary rules.
+Import uPred.
+
+Section CG_Counter.
+  Context {Σ : gFunctors} {iS : cfgSG Σ} {iI : heapIG Σ}.
+
+  (* Coarse-grained increment *)
+  Definition CG_increment (x : expr) : expr :=
+    Lam (App (Lam (Store x.[ren (+ 4)] (NBOP Add (♯ 1) (Var 1))))
+             (Load x.[ren (+ 2)])).
+
+  Lemma CG_increment_type x Γ :
+    typed Γ x (Tref TNat) →
+    typed Γ (CG_increment x) (TArrow TUnit TUnit).
+  Proof.
+    intros H1. repeat econstructor.
+    eapply (context_weakening [_; _; _; _]); eauto.
+    eapply (context_weakening [_; _]); eauto.
+  Qed.
+
+  Lemma CG_increment_closed (x : expr) :
+    (∀ f, x.[f] = x) → ∀ f, (CG_increment x).[f] = CG_increment x.
+  Proof. intros H f. unfold CG_increment. asimpl. rewrite ?H; trivial. Qed.
+
+  Lemma CG_increment_subst (x : expr) f :
+  (CG_increment x).[f] = CG_increment x.[f].
+  Proof. unfold CG_increment; asimpl; trivial. Qed.
+
+  Lemma steps_CG_increment N E ρ j K x n:
+    nclose N ⊆ E →
+    ((Spec_ctx N ρ ★ x ↦ₛ (♯v n) ★
+               j ⤇ (fill K (App (CG_increment (Loc x)) Unit)))%I)
+      ⊢ |={E}=>(j ⤇ (fill K (Unit)) ★ x ↦ₛ (♯v (S n)))%I.
+  Proof.
+    intros HNE. iIntros "[#Hspec [Hx Hj]]". unfold CG_increment.
+    iPvs (step_lam _ _ _ j K _ _ _ _ with "[Hj]") as "Hj"; eauto.
+    iFrame "Hspec Hj"; trivial. simpl.
+    Unshelve. 3: simpl; auto. asimpl.
+    iPvs (step_load _ _ _ j (K ++ [AppRCtx (LamV _)])
+                    _ _ _ with "[Hj Hx]") as "[Hj Hx]"; eauto.
+    rewrite ?fill_app. simpl.
+    iFrame "Hspec Hj"; trivial.
+    rewrite ?fill_app. simpl.
+    iPvs (step_lam _ _ _ j K _ _ _ _ with "[Hj]") as "Hj"; eauto.
+    iFrame "Hspec Hj"; trivial. simpl.
+    Unshelve. 3: simpl; auto.
+    iPvs (step_nat_bin_op _ _ _ j (K ++ [StoreRCtx (LocV _)])
+                          _ _ _  with "[Hj]") as "Hj"; eauto.
+    rewrite ?fill_app. simpl.
+    iFrame "Hspec Hj"; trivial. simpl.
+    rewrite ?fill_app. simpl.
+    iPvs (step_store _ _ _ j K _ _ _ _ _
+          with "[Hj Hx]") as "[Hj Hx]"; eauto.
+    iFrame "Hspec Hj"; trivial.
+    Unshelve. 3: trivial.
+    iPvsIntro.
+    iFrame "Hj Hx"; trivial.
+  Qed.
+
+  Global Opaque CG_increment.
+
+  Definition CG_locked_increment (x l : expr) :=
+    Lam (with_lock (CG_increment x.[ren (+2)]) l.[ren (+2)]).
+  Definition CG_locked_incrementV (x l : expr) : val :=
+    LamV (with_lock (CG_increment x.[ren (+2)]) l.[ren (+2)]).
+
+  Lemma CG_locked_increment_to_val x l :
+    to_val (CG_locked_increment x l) = Some (CG_locked_incrementV x l).
+  Proof. trivial. Qed.
+
+  Lemma CG_locked_increment_of_val x l :
+    of_val (CG_locked_incrementV x l) = CG_locked_increment x l.
+  Proof. trivial. Qed.
+
+  Global Opaque CG_locked_incrementV.
+
+  Lemma CG_locked_increment_type x l Γ :
+    typed Γ x (Tref TNat) →
+    typed Γ l LockType →
+    typed Γ (CG_locked_increment x l) (TArrow TUnit TUnit).
+  Proof.
+    intros H1 H2. repeat econstructor.
+    eapply with_lock_type.
+    - apply CG_increment_type. by eapply (context_weakening [_; _]).
+    - by eapply (context_weakening [_; _]).
+  Qed.
+
+  Lemma CG_locked_increment_closed (x l : expr) :
+    (∀ f, x.[f] = x) → (∀ f, l.[f] = l) →
+    ∀ f, (CG_locked_increment x l).[f] = CG_locked_increment x l.
+  Proof.
+    intros H1 H2 f. asimpl. unfold CG_locked_increment. rewrite H1 H2.
+    rewrite with_lock_closed; trivial. apply CG_increment_closed; trivial.
+  Qed.
+
+  Lemma CG_locked_increment_subst (x l : expr) f :
+  (CG_locked_increment x l).[f] = CG_locked_increment x.[f] l.[f].
+  Proof.
+    unfold CG_locked_increment. simpl.
+    rewrite with_lock_subst CG_increment_subst. asimpl; trivial.
+  Qed.
+
+  Lemma steps_CG_locked_increment N E ρ j K x n l :
+    nclose N ⊆ E →
+    ((Spec_ctx N ρ ★ x ↦ₛ (♯v n) ★ l ↦ₛ (♭v false)
+               ★ j ⤇ (fill K (App
+                                (CG_locked_increment (Loc x) (Loc l)) Unit)))%I)
+      ⊢ |={E}=>(j ⤇ (fill K (Unit)) ★ x ↦ₛ (♯v S n) ★ l ↦ₛ (♭v false))%I.
+  Proof.
+    intros HNE. iIntros "[#Hspec [Hx [Hl Hj]]]". unfold CG_locked_increment.
+    iPvs (step_lam _ _ _ j K _ _ _ _ with "[Hj]") as "Hj"; eauto.
+    iFrame "Hspec Hj"; trivial.
+    rewrite with_lock_closed; auto.
+    iPvs (steps_with_lock
+            _ _ _ j K _ _ _ _ _ _ with "[Hj Hx Hl]") as "Hj"; eauto.
+    - exists UnitV. intros K'.
+      iIntros "[#Hspec [Hx Hj]]".
+      iApply steps_CG_increment; eauto. iFrame "Hspec Hj Hx"; trivial.
+    - iFrame "Hspec Hj Hx"; trivial.
+      Unshelve. all: trivial.
+  Qed.
+
+  Global Opaque CG_locked_increment.
+
+  Definition counter_read (x : expr) : expr := (Lam (Load x.[ren (+2)])).
+  Definition counter_readV (x : expr) : val := (LamV (Load x.[ren (+2)])).
+
+  Lemma counter_read_to_val x: to_val (counter_read x) = Some (counter_readV x).
+  Proof. trivial. Qed.
+
+  Lemma counter_read_of_val x: of_val (counter_readV x) = counter_read x.
+  Proof. trivial. Qed.
+
+  Global Opaque counter_readV.
+
+  Lemma counter_read_type x Γ :
+    typed Γ x (Tref TNat) →
+    typed Γ (counter_read x) (TArrow TUnit TNat).
+  Proof.
+    intros H1. repeat econstructor.
+    eapply (context_weakening [_; _]); trivial.
+  Qed.
+
+  Lemma counter_read_closed (x : expr) :
+    (∀ f, x.[f] = x) →
+    ∀ f, (counter_read x).[f] = counter_read x.
+  Proof. intros H1 f. asimpl. unfold counter_read. by rewrite ?H1. Qed.
+
+  Lemma counter_read_subst (x: expr) f :
+  (counter_read x).[f] = counter_read x.[f].
+  Proof. unfold counter_read. by asimpl. Qed.
+
+  Lemma steps_counter_read N E ρ j K x n :
+    nclose N ⊆ E →
+    ((Spec_ctx N ρ ★ x ↦ₛ (♯v n)
+               ★ j ⤇ (fill K (App (counter_read (Loc x)) Unit)))%I)
+      ⊢ |={E}=>(j ⤇ (fill K (♯ n)) ★ x ↦ₛ (♯v n))%I.
+  Proof.
+    intros HNE. iIntros "[#Hspec [Hx Hj]]". unfold counter_read.
+    iPvs (step_lam _ _ _ j K _ _ _ _ with "[Hj]") as "Hj"; eauto.
+    iFrame "Hspec Hj"; trivial. asimpl.
+    iPvs (step_load _ _ _ j K _ _ _ _ with "[Hj Hx]") as "[Hj Hx]"; eauto.
+    iFrame "Hspec Hj"; trivial.
+    iPvsIntro. iFrame "Hj Hx"; trivial.
+    Unshelve. all: trivial.
+  Qed.
+
+  Opaque counter_read.
+
+  Definition CG_counter_body (x l : expr) : expr :=
+    Pair (CG_locked_increment x l) (counter_read x).
+
+  Lemma CG_counter_body_type x l Γ :
+    typed Γ x (Tref TNat) →
+    typed Γ l LockType →
+    typed Γ (CG_counter_body x l)
+          (TProd (TArrow TUnit TUnit) (TArrow TUnit TNat)).
+  Proof.
+    intros H1 H2; repeat econstructor;
+      eauto using CG_locked_increment_type, counter_read_type.
+  Qed.
+
+  Lemma CG_counter_body_closed (x l : expr) :
+    (∀ f, x.[f] = x) →
+    (∀ f, l.[f] = l) →
+    ∀ f, (CG_counter_body x l).[f] = CG_counter_body x l.
+  Proof.
+    intros H1 H2 f. asimpl.
+    rewrite CG_locked_increment_closed; trivial. by rewrite counter_read_closed.
+  Qed.
+
+  Definition CG_counter : expr :=
+    App (Lam (App (Lam (CG_counter_body (Var 1) (Var 3)))
+                  (Alloc (♯ 0)))) newlock.
+
+  Lemma CG_counter_type Γ :
+    typed Γ CG_counter (TProd (TArrow TUnit TUnit) (TArrow TUnit TNat)).
+  Proof.
+    econstructor; eauto using newlock_type.
+    do 2 econstructor; [|do 2 constructor].
+    constructor. apply CG_counter_body_type; by constructor.
+  Qed.
+
+  Lemma CG_counter_closed f :
+    CG_counter.[f] = CG_counter.
+  Proof.
+    asimpl; rewrite CG_locked_increment_subst counter_read_subst; by asimpl.
+  Qed.
+
+  (* Fine-grained increment *)
+  Definition FG_increment (x : expr) : expr :=
+    Lam (App (Lam
+                (* try increment *)
+                (If (CAS x.[ren (+4)] (Var 1) (NBOP Add (♯ 1) (Var 1)))
+                    Unit (* increment succeeds we return unit *)
+                    (App (Var 2) (Var 3)) (* increment fails, we try again *)
+                )
+             )
+             (Load x.[ren (+2)]) (* read the counter *)
+        ).
+
+  Lemma FG_increment_type x Γ :
+    typed Γ x (Tref TNat) →
+    typed Γ (FG_increment x) (TArrow TUnit TUnit).
+  Proof.
+    intros H1. do 3 econstructor.
+    do 2 econstructor; eauto using EqTNat.
+    - eapply (context_weakening [_; _; _; _]); eauto.
+    - by constructor.
+    - repeat constructor.
+    - by constructor.
+    - by constructor.
+    - eapply (context_weakening [_; _]); eauto.
+  Qed.
+
+  Lemma FG_increment_closed (x : expr) :
+    (∀ f, x.[f] = x) → ∀ f, (FG_increment x).[f] = FG_increment x.
+  Proof. intros H f. asimpl. unfold FG_increment. rewrite ?H; trivial. Qed.
+
+  Definition FG_counter_body (x : expr) : expr :=
+    Pair (FG_increment x) (counter_read x).
+
+  Lemma FG_counter_body_type x Γ :
+    typed Γ x (Tref TNat) →
+    typed Γ (FG_counter_body x)
+          (TProd (TArrow TUnit TUnit) (TArrow TUnit TNat)).
+  Proof.
+    intros H1; econstructor.
+    - apply FG_increment_type; trivial.
+    - apply counter_read_type; trivial.
+  Qed.
+
+  Lemma FG_counter_body_closed (x : expr) :
+    (∀ f, x.[f] = x) →
+    ∀ f, (FG_counter_body x).[f] = FG_counter_body x.
+  Proof.
+    intros H1 f. asimpl. unfold FG_counter_body, FG_increment.
+    rewrite ?H1. by rewrite counter_read_closed.
+  Qed.
+
+  Definition FG_counter : expr :=
+    App (Lam (FG_counter_body (Var 1))) (Alloc (♯ 0)).
+
+  Lemma FG_counter_type Γ :
+    typed Γ FG_counter (TProd (TArrow TUnit TUnit) (TArrow TUnit TNat)).
+  Proof.
+    econstructor; eauto using newlock_type, typed.
+    constructor. apply FG_counter_body_type; by constructor.
+  Qed.
+
+  Lemma FG_counter_closed f :
+    FG_counter.[f] = FG_counter.
+  Proof. asimpl; rewrite counter_read_subst; by asimpl. Qed.
+
+  Ltac prove_disj N n n' :=
+    let Hneq := fresh "Hneq" in
+    let Hdsj := fresh "Hdsj" in
+    assert (Hneq : n ≠ n') by omega;
+    set (Hdsj := ndot_ne_disjoint N n n' Hneq); set_solver_ndisj.
+
+  Lemma FG_CG_counter_refinement N Δ
+        {HΔ : context_interp_Persistent Δ}
+    :
+      (@bin_log_related _ _ _ N Δ [] FG_counter CG_counter
+                        (TProd (TArrow TUnit TUnit) (TArrow TUnit TNat)) HΔ).
+  Proof.
+    (* executing the preambles *)
+    intros vs Hlen. destruct vs; [|inversion Hlen].
+    cbn -[FG_counter CG_counter].
+    intros ρ j K. iIntros "[#Hheap [#Hspec [_ Hj]]]".
+    rewrite ?empty_env_subst.
+    unfold CG_counter, FG_counter.
+    iPvs (steps_newlock _ _ _ j (K ++ [AppRCtx (LamV _)]) _ with "[Hj]")
+      as {l} "[Hj Hl]"; eauto.
+    rewrite fill_app; simpl.
+    iFrame "Hspec Hj"; trivial.
+    rewrite fill_app; simpl.
+    iPvs (step_lam _ _ _ j K _ _ _ _ with "[Hj]") as "Hj"; eauto.
+    iFrame "Hspec Hj"; trivial. simpl.
+    asimpl. rewrite CG_locked_increment_subst; simpl.
+    rewrite counter_read_subst; simpl.
+    iPvs (step_alloc _ _ _ j (K ++ [AppRCtx (LamV _)]) _ _ _ _ with "[Hj]")
+      as {cnt'} "[Hj Hcnt']"; eauto.
+    rewrite fill_app; simpl.
+    iFrame "Hspec Hj"; trivial.
+    rewrite fill_app; simpl.
+    iPvs (step_lam _ _ _ j K _ _ _ _ with "[Hj]") as "Hj"; eauto.
+    iFrame "Hspec Hj"; trivial. simpl.
+    asimpl. rewrite CG_locked_increment_subst; simpl.
+    rewrite counter_read_subst; simpl.
+    Unshelve.
+    all: try match goal with |- to_val _ = _ => auto using to_of_val end.
+    all: trivial.
+    iApply (@wp_bind _ _ _ [AppRCtx (LamV _)]);
+      iApply wp_wand_l; iSplitR; [iIntros {v} "Hv"; iExact "Hv"|].
+    iApply wp_alloc; trivial; iFrame "Hheap"; iNext; iIntros {cnt} "Hcnt".
+    simpl.
+    (* establishing the invariant *)
+    iAssert ((∃ n, l ↦ₛ (♭v false) ★ cnt ↦ᵢ (♯v n) ★ cnt' ↦ₛ (♯v n) )%I)
+      as "Hinv" with "[Hl Hcnt Hcnt']".
+    { iExists _. iFrame "Hl Hcnt Hcnt'"; trivial. }
+    iPvs (inv_alloc (N .@ 4) with "[Hinv]") as "#Hinv"; trivial.
+    { iNext; iExact "Hinv". }
+    (* splitting increment and read *)
+    iApply wp_lam; trivial. iNext. asimpl.
+    rewrite counter_read_subst; simpl.
+    iApply wp_value; simpl.
+    { rewrite counter_read_to_val; trivial. }
+    iExists (PairV (CG_locked_incrementV _ _) (counter_readV _)).
+    simpl. rewrite CG_locked_increment_of_val counter_read_of_val.
+    iFrame "Hj".
+    iExists (_, _), (_, _). simpl; repeat iSplit; trivial.
+    - (* refinement of increment *)
+      iAlways. clear j K. iIntros {j K v} "[#Heq Hj]".
+      rewrite CG_locked_increment_of_val. simpl.
+      iTimeless "Heq". destruct v; iDestruct "Heq" as "[% %]"; simpl in *;subst.
+      iLöb as "Hlat".
+      iApply wp_lam; trivial. asimpl.
+      iNext.
+      (* fine-grained reads the counter *)
+      iApply (@wp_bind _ _ _ [AppRCtx (LamV _)]);
+        iApply wp_wand_l; iSplitR; [iIntros {v} "Hv"; iExact "Hv"|].
+      iInv> (N .@4) as {n} "[Hl [Hcnt Hcnt']]".
+      iApply wp_load; [|iFrame "Hheap"].
+      { prove_disj N 2 4. }
+      iNext; iFrame "Hcnt"; iIntros "Hcnt".
+      iSplitL "Hl Hcnt Hcnt'"; [iExists _; iFrame "Hl Hcnt Hcnt'"; trivial|].
+      iApply wp_lam; trivial. asimpl. iNext.
+      (* fine-grained performs increment *)
+      iApply (@wp_bind _ _ _ [IfCtx _ _; CasRCtx (LocV _) (NatV _)]);
+        iApply wp_wand_l; iSplitR; [iIntros {v} "Hv"; iExact "Hv"|].
+      iApply wp_nat_bin_op; simpl.
+      iNext.
+      iApply (@wp_bind _ _ _ [IfCtx _ _]);
+        iApply wp_wand_l; iSplitR; [iIntros {v} "Hv"; iExact "Hv"|].
+      iInv> (N .@4) as {n'} "[Hl [Hcnt Hcnt']]".
+      (* performing CAS *)
+      destruct (eq_nat_dec n n') as [|Hneq]; subst.
+      + (* CAS succeeds *)
+        (* In this case, we perform increment in the coarse-grained one *)
+        iPvs (steps_CG_locked_increment
+                _ _ _ _ _ _ _ _ _ with "[Hj Hl Hcnt']") as "[Hj [Hcnt' Hl]]".
+        { iFrame "Hspec Hcnt' Hl Hj"; trivial. }
+        iApply wp_cas_suc; simpl; trivial; [|iFrame "Hheap"].
+        { prove_disj N 2 4. }
+        iNext; iFrame "Hcnt"; iIntros "Hcnt".
+        iSplitL "Hl Hcnt Hcnt'"; [iExists _; iFrame "Hl Hcnt Hcnt'"; trivial|].
+        iApply wp_if_true. iNext. iApply wp_value; trivial.
+        iExists _; iSplitL; [|iSplit]; trivial. simpl; trivial.
+      + (* CAS fails *)
+        (* In this case, we perform a recursive call *)
+        iApply (wp_cas_fail _ _ _ _ (♯v n')); simpl; trivial;
+        [inversion 1; subst; auto | | iFrame "Hheap"].
+        { prove_disj N 2 4. }
+        iNext; iFrame "Hcnt"; iIntros "Hcnt".
+        iSplitL "Hl Hcnt Hcnt'"; [iExists _; iFrame "Hl Hcnt Hcnt'"; trivial|].
+        iApply wp_if_false. iNext. iApply "Hlat". iNext; trivial.
+    - (* refinement of read *)
+      iAlways. clear j K. iIntros {j K v} "[#Heq Hj]".
+      rewrite ?counter_read_of_val.
+      iTimeless "Heq". destruct v; iDestruct "Heq" as "[% %]".
+      simpl in *; subst; simpl.
+      Transparent counter_read.
+      unfold counter_read at 2.
+      iApply wp_lam; trivial. simpl.
+      iNext.
+      iInv> (N .@4) as {n} "[Hl [Hcnt Hcnt']]".
+      iPvs (steps_counter_read
+              _ _ _ _ _ _ _ _ with "[Hj Hcnt']") as "[Hj Hcnt']".
+      { by iFrame "Hspec Hcnt' Hj". }
+      iApply wp_load; [|iFrame "Hheap"].
+      { prove_disj N 2 4. }
+      iNext. iFrame "Hcnt"; iIntros "Hcnt".
+      iSplitL "Hl Hcnt Hcnt'"; [iExists _; iFrame "Hl Hcnt Hcnt'"; trivial|].
+      iExists (♯v _); iFrame "Hj". iExists _; by iSplit.
+      Unshelve.
+      all: prove_disj N 3 4.
+  Qed.
+
+End CG_Counter.
